theories/ordinals/Ackermann/PAconsistent.v
@@ -28,12 +28,12 @@ Proof.
     generalize n; clear n.
     induction
       (List.nodup  eq_nat_dec
-         (List.app (freeVarFormula LNT (substituteFormula LNT x0 x1 Zero))
+         (List.app (freeVarFormula LNT (substF LNT x0 x1 Zero))
             (List.app
                (List.remove  eq_nat_dec x1
                   (List.app (freeVarFormula LNT x0)
                      (freeVarFormula LNT
-                        (substituteFormula LNT x0 x1 (Succ (var x1))))))
+                        (substF LNT x0 x1 (Succ (var x1))))))
                (List.remove eq_nat_dec x1 
                   (freeVarFormula LNT x0)))));
       intros n.
